rewrite Compiler2.v

Compiler2.v
@@ -7,25 +7,13 @@ Local Open Scope Z_scope.
 Local Open Scope list_scope.
 Import ListNotations.
 
-Fixpoint is_in_Z (a: Z) (l: list Z) : bool :=
-  match l with
-    | [] => false
-    | b :: m => Z.eqb b a || is_in_Z a m
-  end.
-
-Fixpoint remove_dupsZ (l: list Z) :=
-  match l with
-    | [] => []
-    | x :: xs => if (is_in_Z x xs) then remove_dupsZ xs else x :: remove_dupsZ xs
-  end.
-
 Fixpoint exec_n (l: list instr) (c1: config) (n: nat) (c2: config): Prop :=
   match n with
     | O   => c1 = c2
     | S m => exists c', (exec1 l c1 c') /\ (exec_n l c' m c2)
   end.
 
-Definition _isuccs (i: instr) (n: Z): list Z  :=
+Definition isuccs (i: instr) (n: Z): list Z  :=
   match i with
     | JMP j     => [n + 1 + j]
     | JMPLESS j => [n + 1 + j; n + 1]
@@ -33,561 +21,168 @@ Definition _isuccs (i: instr) (n: Z): list Z  :=
     | _         => [n + 1]
   end.
 
-Definition isuccs i n := remove_dupsZ (_isuccs i n).
+Definition IsSucc (P : list instr) (n : Z) (s : Z) : Prop :=
+  exists i, 0 <= i /\ i < size P /\ List.In s (isuccs (znth i P ADD) (n+i)).
 
-Definition ascii_eqb (a b: Ascii.ascii) :=
-  match a, b with
-    | Ascii.Ascii a1 a2 a3 a4 a5 a6 a7 a8, Ascii.Ascii b1 b2 b3 b4 b5 b6 b7 b8 =>
-      Bool.eqb a1 b1 && 
-      Bool.eqb a2 b2 &&
-      Bool.eqb a3 b3 &&
-      Bool.eqb a4 b4 &&
-      Bool.eqb a5 b5 &&
-      Bool.eqb a6 b6 &&
-      Bool.eqb a7 b7 &&
-      Bool.eqb a8 b8
-  end.
-
-Lemma ascii_eqb_refl: forall a, ascii_eqb a a = true.
-Proof. intros.
-       induction a; intros.
-       simpl.
-       now repeat rewrite eqb_reflx.
-Qed.
-
-Fixpoint string_eqb (x y: string) :=
-  match x, y with
-    | ""%string, ""%string => true
-    | String a s1, String b s2 => 
-      if ascii_eqb a b then
-      string_eqb s1 s2 else false 
-    | _, _ => false
-  end.
-
-Lemma string_eqb_refl: forall x, string_eqb x x = true.
-Proof. intros.
-       induction x; intros.
-       - now simpl. 
-       - simpl. now rewrite ascii_eqb_refl.
-Qed.
-
-
-Fixpoint instr_eqb (i1 i2: instr): bool :=
-  match i1, i2 with
-    | JMP i, JMP j         => Z.eqb i j
-    | LOAD x, LOAD y       => string_eqb x y
-    | LOADI i, LOADI j     => Z.eqb i j
-    | ADD, ADD             => true
-    | STORE x, STORE y     => string_eqb x y
-    | JMPLESS i, JMPLESS j => Z.eqb i j
-    | JMPGE i, JMPGE j     => Z.eqb i j
-    | _, _                 => false
-  end.
-
-Definition succs (P: list instr) (n: Z)
-                 (exprf: { i: Z | (Z.le 0 i) /\ (i < size P)}): list Z :=
- isuccs (znth (proj1_sig exprf) P ADD) (n + (proj1_sig exprf)).
-
-Fixpoint seq (start:Z) (len:nat): list Z :=
-  match len with
-    | O => nil
-    | S len => start :: seq (Z.succ start) len
-  end.
-
-Definition seqZ (n: Z) (m: nat) := seq n (Z.to_nat ((Z.of_nat m) - n)).
-
-Definition exits (P: list instr) exprf: list Z :=
-  let l1   := succs P 0 exprf in
-  let l2   := seqZ 0 (List.length P) in
-  (List.filter (fun a => negb (is_in_Z a l1)) l2).
+Definition IsExit (P : list instr) (s : Z) : Prop :=
+  IsSucc P 0 s /\ ~(0 <= s /\ s < size P).
 
 Section BP_term_exec_n.
+
+Lemma exec_n_exec: forall n P c1 c2,
+    exec_n P c1 n c2 -> exec P c1 c2.
+Proof.
+  induction n; pose @star_step; ycrush.
+Qed.
 
 Lemma exec_0: forall P c, exec_n P c 0 c.
 Proof. scrush. Qed.
 
 Lemma exec_Suc: forall n P c1 c2 c3, exec1 P c1 c2 -> exec_n P c2 n c3 -> exec_n P c1 (S n) c3.
-Proof. intros. simpl.
-       exists c2. scrush.
-Qed.
-
-Lemma exec_n_exec: forall n P c1 c2,
-exec_n P c1 n c2 -> exec P c1 c2.
-Proof. induction n; intros; destruct H.
-- scrush. 
-- pose @star_step;
-Reconstr.hobvious (@H, @IHn)
-(@Star.star_step)
-(@Compiler.exec). Qed.
+Proof. scrush. Qed.
 
 Lemma exec_exec_n: forall P c1 c2,
-exec P c1 c2 ->exists n, exec_n P c1 n c2.
-Proof. intros; induction H.
-- exists O; scrush. 
-- pose exec_Suc; scrush. Qed.
+    exec P c1 c2 ->exists n, exec_n P c1 n c2.
+Proof.
+  intros P c1 c2 H; induction H.
+  - exists O; scrush. 
+  - pose exec_Suc; scrush.
+Qed.
 
 Lemma exec_eq_exec_n: forall P c1 c2, 
-exec P c1 c2 <-> exists n, exec_n P c1 n c2.
-Proof. pose exec_exec_n; 
-pose exec_n_exec; scrush. Qed.
+    exec P c1 c2 <-> exists n, exec_n P c1 n c2.
+Proof.
+  pose exec_exec_n; pose exec_n_exec; scrush.
+Qed.
 
+Lemma exec_n_Nil: forall k c1 c2, exec_n [] c1 k c2 <-> (c1 = c2 /\ k = O).
+Proof.
+  induction k; sauto.
+Qed.
 
 Lemma exec1_exec_n: forall P c1 c2, exec1 P c1 c2 <-> exec_n P c1 1 c2.
 Proof. scrush. Qed.
 
-Lemma exec_trans: forall P c1 c2 c3, exec P c1 c2 -> exec P c2 c3 -> exec P c1 c3.
-Proof. intros.
-       revert c3 H0.
-       induction H; intros;
-       [ scrush |
-        	Reconstr.hobvious (@H, @H1, @IHstar)
-		     (@Star.star_step)
-		     (@Compiler.exec) (** *hammer *)].
+Lemma exec1_exec: forall P c1 c2, exec1 P c1 c2 -> exec P c1 c2.
+Proof.
+  intros.
+  apply exec_n_exec with (n := 1%nat).
+  apply exec1_exec_n.
+  auto.
 Qed.
-
-Lemma exec_n_Nil_l: forall k c1 c2, exec_n [] c1 k c2 -> (c1 = c2 /\ k = O).
-Proof. intro k.
-       induction k; intros; scrush.
-Qed.
-
-Lemma exec_n_Nil_r: forall k c1 c2, (c1 = c2 /\ k = O) -> exec_n [] c1 k c2.
-Proof. intro k.
-       induction k; intros; scrush.
-Qed.
-
-Lemma exec_n_Nil: forall k c1 c2, exec_n [] c1 k c2 <-> (c1 = c2 /\ k = O).
-Proof. pose exec_n_Nil_l; pose exec_n_Nil_r; scrush. Qed.
-
-Lemma exec_n_step_l: forall k n n' P s s' stk stk',
-  n <> n' -> 
-  exec_n P (n, stk, s) k (n', stk', s') -> exists c, exec P (n, stk, s) c /\ exec_n P c (k - 1) (n', stk', s') /\ Nat.lt 0%nat k.
-Proof. intro k.
-       induction k; intros.
-       - cbn in *.
-         exists (n', stk', s'); scrush.
-       - cbn in *. destruct H0. exists x. split.
-         destruct H0.
-         unfold exec.
-         eapply @star_step with (z := x) in H0. 
-         scrush.
-         scrush.
-         assert ((k - 0)%nat = k) by scrush.
-         rewrite H1. split.
-         scrush.
-
-	     Reconstr.htrivial Reconstr.Empty
-		   (@Coq.Arith.PeanoNat.Nat.lt_0_succ, @Coq.Arith.PeanoNat.Nat.le_succ_l)
-		   (@Coq.Arith.PeanoNat.Nat.lt); Reconstr.scrush (** hammer *).
-Qed.
-
-
-Lemma exec1_n_step_l: forall k n n' P s s' stk stk',
-  n <> n' -> 
-  exec_n P (n, stk, s) k (n', stk', s') -> exists c, exec1 P (n, stk, s) c /\ exec_n P c (k - 1) (n', stk', s') /\ Nat.lt 0%nat k.
-Proof. intro k.
-       induction k; intros.
-       - cbn in *.
-         exists (n', stk', s'); scrush.
-       - cbn in *. destruct H0. exists x.
-         destruct H0. split. scrush.
-         split. scrush.
-	       Reconstr.htrivial Reconstr.Empty
-		     (@Coq.Arith.PeanoNat.Nat.lt_0_succ)
-		     (@Coq.Arith.PeanoNat.Nat.lt); scrush.
-Qed.
-
-
-Lemma exec_n_step_r: forall k n n' P s s' stk stk',
-  n <> n' -> 
-  (exists c, exec1 P (n, stk, s) c /\ exec_n P c (k - 1) (n', stk', s') /\ Nat.lt 0%nat k) ->
-   exec_n P (n, stk, s) k (n', stk', s').
-Proof. intros.
-       case_eq k; intros.
-       - destruct H0, H0, H2. subst.
-         contradict H3. scrush.
-       - simpl. destruct H0, H0, H2.
-         exists x. split. easy.
-         assert ((S n0 - 1)%nat = n0) by scrush. subst.
-         now rewrite <- H4.
-Qed.
-
-End BP_term_exec_n.
-
-Section CSES.
 
 Lemma exec_n_step: forall k n n' P s s' stk stk',
-  n <> n' ->
-  (exists c, exec1 P (n, stk, s) c /\ exec_n P c (k - 1) (n', stk', s') /\ Nat.lt 0%nat k) <-> 
-  exec_n P (n, stk, s) k (n', stk', s').
-Proof. split; intros. 
-       pose exec_n_step_r; scrush.
-       pose exec1_n_step_l; scrush.
+  n <> n' -> 
+  exec_n P (n, stk, s) k (n', stk', s') <->
+  exists c, exec1 P (n, stk, s) c /\ exec_n P c (k - 1) (n', stk', s') /\ Nat.lt 0%nat k.
+Proof.
+  destruct k.
+  - sauto.
+  - unfold exec_n; fold exec_n; split; intro; simp_hyps.
+    + assert (HH: (S k - 1)%nat = k) by omega.
+      rewrite HH; clear HH.
+      exists c'.
+      eauto with arith.
+    + assert (HH: (S k - 1)%nat = k) by omega.
+      rewrite HH in *; clear HH.
+      exists c; auto.
+Qed.
+
+Lemma exec1_end: forall P c1 c2, size P <= (fst (fst c1)) -> ~(exec1 P c1 c2).
+Proof.
+  Reconstr.hobvious Reconstr.AllHyps
+		    (@Coq.ZArith.BinInt.Z.lt_nge)
+		    (@Coq.ZArith.BinInt.Z.lt).
 Qed.
 
 Lemma exec_n_end: forall k n n' P s s' stk stk',
   size P <= n -> exec_n P (n, s, stk) k (n', s', stk') -> (n' = n /\ stk' = stk /\ s' = s /\ k = 0%nat).
-Proof. intro k.
-       induction k; intros.
-       - cbn in *; scrush.
-       - cbn in *.
-         destruct H0, H0.
-	       Reconstr.hcrush (@H0, @H)
-		        (@Coq.ZArith.BinInt.Z.lt_nge, @Coq.ZArith.BinInt.Z.gt_lt_iff)
-		        Reconstr.Empty.
+Proof.
+  destruct k.
+  - sauto.
+  - unfold exec_n; fold exec_n; intros; simp_hyps.
+    exfalso; apply exec1_end with (P := P) (c1 := (n, s, stk)) (c2 := c'); scrush.
 Qed.
 
-
-Lemma exec1_end: forall P c1 c2, size P <= (fst (fst c1)) -> (exec1 P c1 c2 -> False).
-Proof. intros.
-       destruct c1, p.
-       cbn in *. unfold exec1 in *.
-       destruct H0, H0, H0, H0.
-       inversion H0. subst.
-       destruct H1, H2.
-       assert ((size P <= x) -> (x < size P) -> False).
-       { Reconstr.hobvious (@H, @H3)
-	       (@Coq.ZArith.BinInt.Z.lt_nge)
-		     Reconstr.Empty.
-       } scrush.
-Qed.
-
-End CSES.
+End BP_term_exec_n.
 
 Section BP_term_succs.
 
-Lemma succs_simps: forall n v x i p, succs [ADD] n p       = remove_dupsZ [n + 1]            /\
-                                     succs [LOADI v] n p   = remove_dupsZ [n + 1]            /\
-                                     succs [LOAD x] n p    = remove_dupsZ [n + 1]            /\
-                                     succs [STORE x] n p   = remove_dupsZ [n + 1]            /\
-                                     succs [JMP i] n p     = remove_dupsZ [n + 1 + i]        /\
-                                     succs [JMPGE i] n p   = remove_dupsZ [n + 1 + i; n + 1] /\
-                                     succs [JMPLESS i] n p = remove_dupsZ [n + 1 + i; n + 1].
-Proof. intros; destruct p; 
-       unfold succs; cbn in *;
-       destruct a;
-       assert (x0 = 0).
-	     { Reconstr.htrivial (@H, @H0)
-		     (@Coq.ZArith.BinInt.Z.lt_succ_r, @Coq.ZArith.BinInt.Z.le_refl, 
-         @Coq.ZArith.BinInt.Z.le_antisymm, @Coq.ZArith.BinInt.Z.log2_up_nonpos, 
-         @Coq.ZArith.BinInt.Z.log2_up_null, @Coq.ZArith.Znat.Z2Nat.inj_0, 
-         @Coq.ZArith.Znat.Z2Nat.inj_succ, @Coq.ZArith.Znat.Z2Nat.inj_lt,
-         @Coq.ZArith.BinInt.Z.one_succ) (@Coq.Arith.PeanoNat.Nat.lt); scrush.
-        } rewrite H1; scrush.
+Lemma succs_simps: forall n v x i,
+    (forall s, IsSucc [ADD] n s <-> s = n + 1) /\
+    (forall s, IsSucc [LOADI v] n s <-> s = n + 1) /\
+    (forall s, IsSucc [LOAD x] n s <-> s = n + 1) /\
+    (forall s, IsSucc [STORE x] n s <-> s = n + 1) /\
+    (forall s, IsSucc [JMP i] n s <-> s = n + 1 + i) /\
+    (forall s, IsSucc [JMPGE i] n s <-> s = n + 1 + i \/ s = n + 1) /\
+    (forall s, IsSucc [JMPLESS i] n s <-> s = n + 1 + i \/ s = n + 1).
+Proof.
+  unfold IsSucc.
+  intros; repeat split; intro; simp_hyps; cbn in *;
+    solve [ assert (i0 = 0) by omega; sauto | exists 0; sauto ].
 Qed.
 
-Lemma succs_empty: forall n p, succs [] n p = [].
-Proof. intros; destruct p; unfold succs; cbn in *;
-	     Reconstr.hobvious (@a)
-		   (@Coq.ZArith.BinInt.Z.lt_nge, @Coq.ZArith.Znat.Z2Nat.inj_lt, @Coq.ZArith.BinInt.Z.le_refl)
-		   Reconstr.Empty.
+Lemma succs_empty: forall n s, ~(IsSucc [] n s).
+Proof.
+  unfold IsSucc.
+  Reconstr.hobvious Reconstr.Empty
+		    (@Coq.ZArith.BinInt.Z.abs_nonneg, @Coq.ZArith.BinInt.Z.le_refl, @Coq.ZArith.BinInt.Z.abs_eq,
+                     @Coq.ZArith.BinInt.Z.ltb_nlt, @Coq.ZArith.BinInt.Z.nle_gt, @Coq.ZArith.BinInt.Z.le_lt_trans)
+		    (@Compiler.size).
 Qed.
 
-Lemma succs_iexec1: forall P s stk c p, c = iexec (znth (proj1_sig p) P ADD) ((proj1_sig p), s, stk) ->
-                                        List.In (fst (fst c)) (succs P 0 p).
-Proof. intros; destruct c, p0, p; unfold succs, isuccs, _isuccs. cbn in *.
-       case_eq (znth x P ADD ); intros; rewrite H0 in *;
-       try scrush.
-       case_eq (hd 0 (tl stk) <? hd 0 stk); intros; rewrite H1 in *; inversion H; try scrush.
-       unfold remove_dupsZ.
-       case_eq (is_in_Z (x + 1 + z0) [x + 1]); intros.
-       inversion H2.
-       assert ((x + 1 =? x + 1 + z0) = true). scrush.
-       assert ((x + 1 = x + 1 + z0)).
-       { Reconstr.htrivial (@H6)
-	     	 (@Coq.ZArith.BinInt.Z.add_1_l, @Coq.ZArith.BinInt.Z.eqb_eq)
-		     (@Coq.ZArith.BinIntDef.Z.succ).
-       }  
-       assert (z0 = 0).
-       { Reconstr.hsimple (@H8)
-		     (@Coq.ZArith.BinInt.Z.add_cancel_l, @Coq.ZArith.BinInt.Z.add_0_r)
-		     Reconstr.Empty.
-       } subst. cbn. scrush.
-       cbn. now left.
-       inversion H. 
-       case_eq (hd 0 (tl stk) >=? hd 0 stk); intros; rewrite H1 in *.
-       inversion H. cbn.
-       case_eq ( (x + 1 =? x + 1 + z0)); intros.
-       assert ((x + 1 = x + 1 + z0)).
-       { Reconstr.htrivial (@H5)
-	     	 (@Coq.ZArith.BinInt.Z.add_1_l, @Coq.ZArith.BinInt.Z.eqb_eq)
-		     (@Coq.ZArith.BinIntDef.Z.succ).
-       }
-       assert (z0 = 0).
-       { Reconstr.hsimple (@H9)
-		     (@Coq.ZArith.BinInt.Z.add_cancel_l, @Coq.ZArith.BinInt.Z.add_0_r)
-		     Reconstr.Empty.
-       } subst. cbn. scrush.
-       scrush.
-       cbn.
-       case_eq ((x + 1 =? x + 1 + z0)); intros.
-       now left.
-       right. scrush.
+Lemma succs_Cons: forall x xs n s,
+    IsSucc (x :: xs) n s <-> List.In s (isuccs x n) \/ IsSucc xs (n + 1) s.
+Proof.
+  split; intro H; unfold IsSucc in H; simp_hyps.
+  - assert (H2: i = 0 \/ i > 0) by
+	Reconstr.hcrush (@H)
+		(@Coq.ZArith.BinInt.Z.lt_eq_cases, @Coq.ZArith.BinInt.Z.lt_nge, @Coq.ZArith.Zorder.Znot_le_gt)
+		Reconstr.Empty.
+    assert (H3: i = 0 \/ exists j, j >= 0 /\ i = j + 1) by
+    (sauto; [
+       Reconstr.hcrush Reconstr.AllHyps
+		    (@Coq.ZArith.BinInt.Z.abs_nonneg, @Coq.ZArith.Znat.Z2Nat.id, @Coq.ZArith.Znat.Z2Nat.inj_0)
+		    (@Coq.ZArith.BinIntDef.Z.abs) |
+       Reconstr.hcrush Reconstr.AllHyps
+		       (@Coq.ZArith.BinInt.Z.le_exists_sub, @Coq.ZArith.BinInt.Z.le_gt_cases, @Coq.ZArith.BinInt.Z.add_0_l, @Coq.ZArith.Zcompare.Zcompare_Gt_not_Lt, @Coq.ZArith.BinInt.Z.ge_le_iff)
+		       (@Coq.ZArith.BinInt.Z.lt) ]).
+    clear H2.
+    destruct H3; simp_hyps.
+    + sauto.
+    + subst; right; unfold IsSucc.
+      exists j.
+      repeat split.
+      * auto with zarith.
+      * Reconstr.hsimple Reconstr.AllHyps
+		         (@Coq.ZArith.BinInt.Z.add_lt_mono_r, @Compiler.lem_size_succ)
+		         Reconstr.Empty.
+      * Reconstr.hcrush Reconstr.AllHyps
+		        (@Coq.ZArith.BinInt.Z.add_comm, @Coq.ZArith.BinInt.Z.ge_le_iff,
+                         @Coq.ZArith.BinInt.Zplus_assoc_reverse, @Compiler.lem_n_succ_znth)
+		        Reconstr.Empty.
+  - destruct H.
+    + unfold IsSucc; exists 0; scrush.
+    + unfold IsSucc; simp_hyps. exists (i + 1).
+      repeat split.
+      * omega.
+      * Reconstr.hcrush Reconstr.AllHyps
+		        (@Coq.ZArith.BinInt.Z.add_lt_mono_r, @Compiler.lem_size_succ)
+		        Reconstr.Empty.
+      * sauto; [
+          Reconstr.hcrush Reconstr.AllHyps
+		          (@Coq.ZArith.Znat.Z2Nat.inj_succ)
+		          (@Coq.ZArith.BinIntDef.Z.succ) |
+	  Reconstr.hcrush Reconstr.AllHyps
+		          (@Coq.ZArith.BinInt.Zplus_assoc_reverse, @Coq.ZArith.BinInt.Z.add_comm, @Coq.ZArith.Znat.Z2Nat.inj_succ, @Coq.ZArith.BinInt.Z.add_succ_l, @Coq.ZArith.BinInt.Z.add_shuffle3)
+		          (@Compiler.znth, @Coq.ZArith.BinIntDef.Z.succ) ].
 Qed.
 
-Lemma In_Singleton: forall {A} (a b: A),  In a [b] -> a = b.
-Proof. intros; destruct H; cbn in *; scrush. Qed.
-
-Lemma succs_shift: forall P n k p, List.In (k - n) (succs P 0 p) -> List.In k (succs P n p).
-Proof. intros.
-       destruct p. cbn in *.
-       unfold succs in *. cbn in *.
-       unfold isuccs in *.
-       case_eq (znth x P ADD ); intros; rewrite H0 in *.
-       apply In_Singleton in H.
-       assert (k = n + x + 1).
-       { 	Reconstr.htrivial (@H)
-		     (@Coq.ZArith.BinInt.Zplus_assoc_reverse, @Coq.ZArith.BinInt.Zplus_minus)
-		      Reconstr.Empty.
-       } scrush.
-       apply In_Singleton in H.
-       assert (k = n + x + 1).
-       { 	Reconstr.htrivial (@H)
-		     (@Coq.ZArith.BinInt.Zplus_assoc_reverse, @Coq.ZArith.BinInt.Zplus_minus)
-		      Reconstr.Empty.
-       } scrush.
-       apply In_Singleton in H.
-       assert (k = n + x + 1).
-       { 	Reconstr.htrivial (@H)
-		     (@Coq.ZArith.BinInt.Zplus_assoc_reverse, @Coq.ZArith.BinInt.Zplus_minus)
-		      Reconstr.Empty.
-       } scrush.
-       apply In_Singleton in H.
-       assert (k = n + x + 1).
-       { 	Reconstr.htrivial (@H)
-		     (@Coq.ZArith.BinInt.Zplus_assoc_reverse, @Coq.ZArith.BinInt.Zplus_minus)
-		      Reconstr.Empty.
-       } scrush.
-       apply In_Singleton in H.
-       assert (k = n + x + 1 + z).
-       { Reconstr.htrivial (@H)
-		     (@Coq.ZArith.BinInt.Zplus_assoc_reverse, @Coq.ZArith.BinInt.Z.add_simpl_r, @Coq.ZArith.BinInt.Zplus_minus)
-		     Reconstr.Empty.
-       } scrush.
-       cbn in *.
-       case_eq ((x + 1 =? x + 1 + z)); intros.
-       assert ((x + 1 = x + 1 + z)).
-       { Reconstr.htrivial (@H1)
-		     (@Coq.ZArith.BinInt.Z.add_1_l, @Coq.ZArith.BinInt.Z.eqb_eq)
-		     (@Coq.ZArith.BinIntDef.Z.succ).
-       }
-       assert (z = 0).
-       { Reconstr.hsimple (@H2)
-		     (@Coq.ZArith.BinInt.Z.add_cancel_l, @Coq.ZArith.BinInt.Z.add_0_r)
-		      Reconstr.Empty; scrush.
-       } subst. cbn.
-       assert (n + x + 1 + 0 = n + x + 1).
-       { scrush. }
-       rewrite H3.
-       assert ((n + x + 1 =? n + x + 1) = true).
-       { Reconstr.htrivial Reconstr.Empty
-		     (@Coq.ZArith.BinInt.Z.eqb_eq)
-		     (@Coq.ZArith.BinIntDef.Z.succ); scrush.
-       }
-       rewrite H4. cbn.
-       assert ((x + 1 =? x + 1 + 0) = true).
-       { scrush. }
-       rewrite H5 in *. cbn in *.
-       assert (k = n + x + 1).
-       { Reconstr.htrivial (@H)
-		     (@Coq.ZArith.BinInt.Zplus_succ_r_reverse, @Coq.ZArith.BinInt.Zplus_minus)
-		     (@Coq.ZArith.BinIntDef.Z.sub, @Coq.ZArith.BinIntDef.Z.succ).
-       } scrush.
-       rewrite H1 in *. cbn in *.
-       assert ((n + x + 1 <> n + x + 1 + z)).
-       { assert (x + 1 <> x + 1 + z).
-         { Reconstr.hcrush (@H1)
-	       	 (@Coq.ZArith.BinInt.Z.add_0_r, @Coq.ZArith.BinInt.Z.eqb_eq, @Coq.ZArith.BinInt.Z.add_cancel_l)
-		       (@Coq.ZArith.BinIntDef.Z.succ).
-         } unfold Logic.not in *. intros.  
-         specialize (Coq.ZArith.BinInt.Z.add_cancel_l (x + 1) (x + 1 + z) n); intros.
-         apply H2. apply H4.	
-        Reconstr.htrivial (@H3)
-		    (@Coq.ZArith.BinInt.Zplus_succ_r_reverse, @Coq.ZArith.BinInt.Zplus_assoc_reverse)
-	      (@Coq.ZArith.BinIntDef.Z.succ).
-       }
-       assert ((n + x + 1 =? n + x + 1 + z) = false).
-       { Reconstr.htrivial (@H2)
-		     (@Coq.ZArith.BinInt.Z.eqb_neq)
-		     Reconstr.Empty.
-       }
-       rename H2 into H2a.
-       rename H3 into H2.
-       rewrite H2. cbn.
-       destruct H. left.
-	     Reconstr.htrivial (@H)
-		   (@Coq.ZArith.BinInt.Zplus_assoc_reverse, @Coq.ZArith.BinInt.Z.add_succ_r, @Coq.ZArith.BinInt.Z.add_simpl_r, @Coq.ZArith.BinInt.Zplus_minus)
-		   (@Coq.ZArith.BinIntDef.Z.sub, @Coq.ZArith.BinIntDef.Z.succ).
-       destruct H.
-       right. left.
-	     Reconstr.htrivial (@H) 
-		   (@Coq.ZArith.BinInt.Z.add_succ_r, @Coq.ZArith.BinInt.Zplus_minus)
-		   (@Coq.ZArith.BinIntDef.Z.succ, @Coq.ZArith.BinIntDef.Z.sub). scrush.
-
-       cbn in *.
-       case_eq ((x + 1 =? x + 1 + z)); intros; rewrite H1 in *; cbn in *.
-       destruct H.
-       assert ( (n + x + 1 =? n + x + 1 + z) = true).
-       { Reconstr.hcrush (@H1)
-		    (@Coq.ZArith.BinInt.Zplus_assoc_reverse, @Coq.ZArith.BinInt.Z.add_succ_r, @Coq.ZArith.BinInt.Z.eqb_eq, @Coq.ZArith.BinInt.Z.eqb_refl)
-		    (@Coq.ZArith.BinIntDef.Z.succ).
-       } rewrite H2. cbn. left. 
-       Reconstr.htrivial (@H)
-       (@Coq.ZArith.BinInt.Zplus_succ_r_reverse, @Coq.ZArith.BinInt.Zplus_minus)
-       (@Coq.ZArith.BinIntDef.Z.succ, @Coq.ZArith.BinIntDef.Z.sub).
-       scrush.
-       assert ((n + x + 1 <> n + x + 1 + z)).
-       { assert (x + 1 <> x + 1 + z).
-         { Reconstr.hcrush (@H1)
-	       	 (@Coq.ZArith.BinInt.Z.add_0_r, @Coq.ZArith.BinInt.Z.eqb_eq, @Coq.ZArith.BinInt.Z.add_cancel_l)
-		       (@Coq.ZArith.BinIntDef.Z.succ).
-         } unfold Logic.not in *. intros.  
-         specialize (Coq.ZArith.BinInt.Z.add_cancel_l (x + 1) (x + 1 + z) n); intros.
-         apply H2. apply H4.	
-        Reconstr.htrivial (@H3)
-		    (@Coq.ZArith.BinInt.Zplus_succ_r_reverse, @Coq.ZArith.BinInt.Zplus_assoc_reverse)
-	      (@Coq.ZArith.BinIntDef.Z.succ).
-       }
-       assert ((n + x + 1 =? n + x + 1 + z) = false).
-       { Reconstr.htrivial (@H2)
-		     (@Coq.ZArith.BinInt.Z.eqb_neq)
-		      Reconstr.Empty. }
-       rename H2 into H2a.
-       rename H3 into H2.
-       rewrite H2. cbn.
-       destruct H. left.
-	     Reconstr.htrivial (@H)
-		   (@Coq.ZArith.BinInt.Zplus_assoc_reverse, @Coq.ZArith.BinInt.Z.add_succ_r, 
-        @Coq.ZArith.BinInt.Z.add_simpl_r, @Coq.ZArith.BinInt.Zplus_minus)
-		   (@Coq.ZArith.BinIntDef.Z.sub, @Coq.ZArith.BinIntDef.Z.succ).
-       destruct H. right.
-	     Reconstr.htrivial (@H)
-		   (@Coq.ZArith.BinInt.Z.add_succ_r, @Coq.ZArith.BinInt.Zplus_minus)
-		   (@Coq.ZArith.BinIntDef.Z.succ, @Coq.ZArith.BinIntDef.Z.sub).
-       scrush.
+Lemma succs_iexec1: forall P n s stk c,
+    0 <= n -> n < size P -> c = iexec (znth n P ADD) (n, s, stk) -> IsSucc P 0 (fst (fst c)).
+Proof.
+  unfold IsSucc; unfold iexec.
+  sauto; exists n; scrush.
 Qed.
-
-Lemma prf_cons: forall (x: instr) (xs: list instr), 
-{i : Z | 0 <= i /\ i < (size xs)} -> 
-{i : Z | 0 <= i /\ i < (size (x :: xs))}.
-Proof. intros. destruct H. exists x0; unfold size in *; cbn in *;
-     	 Reconstr.hobvious (@a)
-		  (@Coq.ZArith.BinInt.Z.lt_succ_r, @Coq.ZArith.Znat.Zpos_P_of_succ_nat)
-		  (@Coq.ZArith.BinInt.Z.lt, @Coq.ZArith.BinInt.Z.le, @Compiler.size).
-Defined.
-
-Lemma succs_Cons: forall x xs n q,
-succs (x :: xs) n (prf_cons x xs q) = remove_dupsZ (isuccs x n ++ succs xs (n + 1) q).
-Proof. intros. unfold succs.
-       cut (exists k, List.In k (succs (x :: xs) n (prf_cons x xs q))); intros.
-       destruct H as (k, H).
-       destruct q as (i, iH).
-       assert ((fun p P n i => 0 <= i /\ i < size P /\ List.In p (isuccs (znth i P ADD) (n + i)))
-       k (x :: xs) n i). split. inversion iH. easy.
-       split. inversion iH.
-	     Reconstr.hcrush (@H1)
-		    (@Coq.ZArith.BinInt.Z.lt_succ_r, @Compiler.lem_size_succ)
-		    (@Coq.ZArith.BinInt.Z.lt, @Coq.ZArith.BinInt.Z.le,
-         @Coq.ZArith.BinIntDef.Z.succ). scrush.
-
-       unfold succs in *. cbn in *.
-       case_eq ( Z.to_nat i); intros.
-       assert (i = 0) by admit.
-Admitted.
-
-
-Lemma helper: forall (xs ys: list instr) a,
-   a < size ys ->
-   a < size (xs ++ ys).
-Proof. intro xs.
-       induction xs; intros.
-       - now cbn.
-       - Reconstr.hsimple (@IHxs, @H)
-		     (@Coq.ZArith.BinInt.Z.lt_succ_r, @Coq.ZArith.Znat.Zpos_P_of_succ_nat, 
-          @Coq.Lists.List.app_length, @Coq.ZArith.BinInt.Z.lt_eq_cases)
-		      (@Compiler.size).
-Qed.
-
-Lemma prf_concat: forall (xs ys: list instr),
-{i : Z | 0 <= i /\ i < size ys} ->
-{i : Z | 0 <= i /\ i < size (xs ++ ys)}. 
-Proof. intros. destruct H. exists x. split. easy.
-       destruct a. now apply helper.
-Defined.
-
-Lemma succs_append: forall xs ys n p q, succs (xs ++ ys) n (prf_concat xs ys p) = 
-                                        succs xs n q ++ succs ys (n + size xs) p.
-Proof. Admitted.
-
-
-(** go through the whole file..! *)
-
 
 End BP_term_succs.
-
-Section Corr.
-
-Lemma not_Nil: forall a b, a ++ b ++ [ADD] <> [].
-Proof. induction a; sauto; scrush. Qed.
-
-Lemma acomq_neq_nil: forall a, acomp a <> [].
-Proof. induction a; try (cbn; easy).
-       pose not_Nil; scrush.
-Qed.
-
-Lemma acomp_exec1_n_h: forall s s' stk stk' v,
-  exec1 [LOADI v] (0, s, stk) (1, s', stk') -> s' = s.
-Proof. scrush. Qed.
-
-
-Lemma acomp_exec_n: forall a n s s' stk stk',
-  exec_n (acomp a) (0, s, stk) n (size (acomp a), s', stk') ->
-  s' = s /\ stk' = (aval s a) :: stk.
-Proof. induction a; intros.
-       - apply exec_n_step in H. destruct H, H, x, p.
-         assert (z = 1). scrush. subst.
-         assert (size [LOADI v] <= 1). scrush.
-         destruct H0.
-         specialize (@exec_n_end (n - 1) 1 1 
-                    [LOADI v] s1 s' s0 stk' H1 H0); intros.
-         assert (s1 = s). scrush.
-         scrush. scrush.
-       - apply exec_n_step in H. destruct H, H, x, p.
-         cbn in *.
-         assert (z = 1). scrush. subst.
-         assert (size [LOAD v] <= 1). scrush.
-         destruct H0.
-         specialize (@exec_n_end (n - 1) 1 1 
-                    [LOAD v] s1 s' s0 stk' H1 H0); intros.
-         assert (s1 = s). scrush.
-         scrush. scrush.
-       - cbn in *.
-         case_eq (Aplus a1 a2); intros.
-         assert ((size (acomp a1 ++ acomp a2 ++ [ADD]) =
-                 (size (acomp a1) + (size (acomp a2) + 1)))) by admit.
-         rewrite H1 in H.
-Admitted.
-
-
-
-End Corr.
-
-
-
-
-
-
-
-
-
-
-
-
-
-
-
-
-
-
-
-
-
